theories/Lambda/ExprDsimpl.v
@@ -5,7 +5,6 @@ Require Import ExtLib.Structures.Functor.
 Require Import ExtLib.Data.HList.
 Require Import ExtLib.Data.List.
 Require Import ExtLib.Data.Eq.
-Require Import ExtLib.Data.Fun.
 Require Import ExtLib.Data.Monads.OptionMonad.
 Require Import ExtLib.Tactics.
 Require Import MirrorCore.EnvI.
