theories/Lambda/ExprSubst.v
@@ -4,7 +4,6 @@
 Require Import Coq.Classes.Morphisms.
 Require Import Coq.omega.Omega.
 Require Import ExtLib.Core.RelDec.
-Require Import ExtLib.Data.Fun.
 Require Import ExtLib.Data.ListNth.
 Require Import ExtLib.Data.HList.
 Require Import ExtLib.Tactics.
@@ -104,7 +103,7 @@ Section instantiate_thm.
   Variable typ : Type.
   Variable func : Type.
   Variable RType_typ : RType typ.
-  Variable Typ2_Fun : Typ2 _ Fun.
+  Variable Typ2_Fun : Typ2 _ RFun.
   Context {RSym_func : RSym func}.
 
   (** Reasoning principles **)
