theories/Lambda/ExprUnify.v
@@ -25,7 +25,7 @@ Section typed.
   Context {RSym_func : RSym func}.
   Context {RSymOk_func : RSymOk RSym_func}.
   Local Existing Instance Expr_expr.
-  Context {Typ2_arr : Typ2 _ Fun}.
+  Context {Typ2_arr : Typ2 _ RFun}.
   Context {Typ2Ok_arr : Typ2Ok Typ2_arr}.
 
   Context {Subst_subst : Subst subst (expr typ func)}.
@@ -108,7 +108,7 @@ Section typed.
           end
         | Abs t1 e1 , Abs t2 e2 =>
           (* t1 = t2 since both terms have the same type *)
-          typ2_match (F := Fun) (fun _ => _) t
+          typ2_match (F:=RFun) (fun _ => _) t
                      (fun _ t =>
                         exprUnify' us (t1 :: vs) (S n) e1 e2 t s)
                      None
