theories/Lambda/ExprUnify_simul.v
@@ -1,7 +1,6 @@
 Require Import ExtLib.Core.RelDec.
 Require Import ExtLib.Data.HList.
 Require Import ExtLib.Data.Option.
-Require Import ExtLib.Data.Fun.
 Require Import ExtLib.Data.Eq.
 Require Import ExtLib.Data.Pair.
 Require Import ExtLib.Tactics.
@@ -30,7 +29,7 @@ Section typed.
   Context {RSym_func : RSym func}.
   Context {RSymOk_func : RSymOk RSym_func}.
   Local Existing Instance Expr_expr.
-  Context {Typ2_arr : Typ2 _ Fun}.
+  Context {Typ2_arr : Typ2 _ RFun}.
   Context {Typ2Ok_arr : Typ2Ok Typ2_arr}.
   Context {Subst_subst : Subst subst (expr typ func)}.
   Context {SubstUpdate_subst : SubstUpdate subst (expr typ func)}.
