theories/Lambda/ExprVariables.v
@@ -1,4 +1,3 @@
-Require Import ExtLib.Data.Fun.
 Require Import ExtLib.Data.HList.
 Require Import ExtLib.Tactics.
 Require Import MirrorCore.OpenT.
@@ -10,7 +9,7 @@ Section parametric.
   Context {typ : Type}.
   Context {func : Type}.
   Context {RType_typD : RType typ}.
-  Context {Typ2_Fun : Typ2 RType_typD Fun}.
+  Context {Typ2_Fun : Typ2 RType_typD RFun}.
   Context {RSym_func : RSym func}.
 
   (** Reasoning principles **)
