theories/Views/ApplicativeView.v
@@ -1,6 +1,5 @@
 Require Import ExtLib.Core.RelDec.
 Require Import ExtLib.Structures.Applicative.
-Require Import ExtLib.Data.Fun.
 Require Import ExtLib.Data.String.
 Require Import ExtLib.Data.Map.FMapPositive.
 Require Import ExtLib.Data.SumN.
@@ -30,17 +29,17 @@ Set Maximal Implicit Insertion.
 Inductive ap_func (typ : Type) :=
 | pPure (_ : typ)
 | pAp (_ _ : typ).
-    
+
 Implicit Arguments ap_func [].
-    
+
 Section ApplicativeFuncInst.
   Context {typ func : Type} {RType_typ : RType typ}.
   Context {Heq : RelDec (@eq typ)} {HC : RelDec_Correct Heq}.
   Context {T : Type -> Type} {Applicative_T : Applicative T}.
 
-  Context {Typ2_tyArr : Typ2 _ Fun}.
+  Context {Typ2_tyArr : Typ2 _ RFun}.
   Context {Typ1_T : Typ1 _ T}.
-    	
+
   Let tyArr : typ -> typ -> typ := @typ2 _ _ _ _.
   Let tyT : typ -> typ := @typ1 _ _ _ _.
 
@@ -67,12 +66,12 @@ Section ApplicativeFuncInst.
   Qed.
 
   Definition pureR t : typD (tyArr t (tyT t)) :=
-    castR id (Fun (typD t) (T (typD t))) (@pure T Applicative_T (typD t)).
+    castR id (RFun (typD t) (T (typD t))) (@pure T Applicative_T (typD t)).
 
   Definition apR t u : typD (tyArr (tyT (tyArr t u)) (tyArr (tyT t) (tyT u))) :=
-    castR id (Fun (T (Fun (typD t) (typD u))) (Fun (T (typD t)) (T (typD u))))
+    castR id (RFun (T (RFun (typD t) (typD u))) (RFun (T (typD t)) (T (typD u))))
           (@ap T Applicative_T (typD t) (typD u)).
-  
+
   Definition ap_func_symD f : match typeof_ap_func f return Type with
 	                      | Some t => typD t
 	                      | None => unit
@@ -84,7 +83,7 @@ Section ApplicativeFuncInst.
     | pPure t => pureR t
     | pAp t u => apR t u
     end.
-      
+
     Global Instance RSym_ApFunc : SymI.RSym (ap_func typ) := {
       typeof_sym := typeof_ap_func;
       symD := ap_func_symD;
@@ -103,8 +102,8 @@ End ApplicativeFuncInst.
 Section MakeApplicative.
   Context {typ func : Type} {RType_typ : RType typ}.
   Context {FV : FuncView func (ap_func typ)}.
-  Context {Typ2_tyArr : Typ2 _ Fun}.
-    	
+  Context {Typ2_tyArr : Typ2 _ RFun}.
+
   Let tyArr : typ -> typ -> typ := @typ2 _ _ _ _.
 
   Definition fPure t := f_insert (pPure t).
@@ -114,7 +113,7 @@ Section MakeApplicative.
   Definition mkAp (t u : typ) (f a : expr typ func) := App (App (Inj (fAp t u)) f) a.
 
   Fixpoint mkAps f es t :=
-    match es with 
+    match es with
     | nil => mkPure t f
     | (e, t')::es => mkAp t' t (mkAps f es (tyArr t' t)) e
     end.
@@ -150,7 +149,7 @@ Section MakeApplicative.
     red; intros.
     destruct x; simpl; [|destruct (Hok (t, t0))].
     { right; unfold Fails; reflexivity. }
-    { left. destruct H; exists x; revert H; compute; intros. 
+    { left. destruct H; exists x; revert H; compute; intros.
       rewrite H. reflexivity. }
     { right; unfold Fails in *; intros; simpl; rewrite H; reflexivity. }
   Qed.
@@ -184,15 +183,15 @@ Section MakeApplicative.
     rewrite H0 in H; inv_all; subst.
     exists t, t0; split; [assumption | reflexivity].
   Qed.
-  
-  Global Instance fptrnPure_SucceedsE {T : Type} {f : ap_func typ} 
+
+  Global Instance fptrnPure_SucceedsE {T : Type} {f : ap_func typ}
          {p : ptrn typ T} {res : T} {pok : ptrn_ok p} :
     SucceedsE f (fptrnPure p) res := {
       s_result := exists t, Succeeds t p res /\ f = pPure t;
       s_elim := @Succeeds_fptrnPure T f p res pok
     }.
 
-  Global Instance fptrnAp_SucceedsE {T : Type} {f : ap_func typ} 
+  Global Instance fptrnAp_SucceedsE {T : Type} {f : ap_func typ}
          {p : ptrn (typ * typ) T} {res : T} {pok : ptrn_ok p} :
     SucceedsE f (fptrnAp p) res := {
       s_result := exists t u, Succeeds (t, u) p res /\ f = pAp t u;
@@ -205,12 +204,12 @@ Section MakeApplicative.
     por (appr (inj (ptrn_view _ (fptrnPure (pmap do_pure Ptrns.get)))) Ptrns.get)
         (appr (appr (inj (ptrn_view _ (fptrnAp (pmap (fun x a b => do_ap (fst x) (snd x) a b)
                                                      Ptrns.get))))
-                    Ptrns.get) 
+                    Ptrns.get)
               Ptrns.get).
 
 Definition applicative_cases {T : Type}
            (do_pure : typ  -> expr typ func -> T)
-           (do_ap : typ -> typ -> expr typ func -> expr typ func -> T) 
+           (do_ap : typ -> typ -> expr typ func -> expr typ func -> T)
            (do_default : T) : Ptrns.tptrn (expr typ func) T :=
   pdefault (applicative_ptrn_cases do_pure do_ap)
            do_default.
@@ -221,7 +220,7 @@ Section PtrnString.
   Context {typ func : Type} {RType_typ : RType typ}.
   Context {FV : FuncView func (ap_func typ)}.
 
-(* Putting this in the previous sectioun caused universe inconsistencies 
+(* Putting this in the previous sectioun caused universe inconsistencies
   when calling '@mkAp typ func' in JavaFunc (with typ and func instantiated) *)
 
   Definition ptrnPure {T A : Type}
@@ -230,7 +229,7 @@ Section PtrnString.
 
   Definition ptrnAp {A B T : Type}
              (p : ptrn (typ * typ) T)
-             (a : ptrn (expr typ func) A) 
+             (a : ptrn (expr typ func) A)
              (b : ptrn (expr typ func) B) : ptrn (expr typ func) (T * A * B) :=
     app (app (inj (ptrn_view _ (fptrnAp p))) a) b.
 
